src/high/or_lost.v
@@ -1,0 +1,185 @@
+From iris.algebra Require Import auth.
+From iris.bi Require Import fractional.
+From iris.proofmode Require Import reduction monpred tactics.
+
+From Perennial.Helpers Require Import ipm NamedProps.
+From Perennial.program_logic Require Import recovery_weakestpre.
+
+From self Require Import extra ipm_tactics.
+From self.algebra Require Import ghost_map.
+From self.base Require Import primitive_laws wpr_lifting.
+From self.high Require Import dprop resources monpred_simpl.
+
+Set Default Proof Using "Type".
+
+Notation base_post_crash := post_crash_modality.post_crash.
+
+Section or_lost_post_crash.
+  Context `{nvmBaseFixedG Σ, nD: nvmBaseDeltaG Σ}.
+
+  Definition or_lost_post_crash ℓ (P : nat → iProp Σ) :=
+    (∃ (CV : view),
+      crashed_at CV ∗
+      ((∃ t, ⌜CV !! ℓ = Some (MaxNat t)⌝ ∗ persisted_loc ℓ 0 ∗ P t)
+      ∨ ⌜CV !! ℓ = None⌝))%I.
+
+  Instance or_lost_post_crash_proper ℓ :
+    Proper (pointwise_relation _ (⊣⊢) ==> (⊣⊢)) (or_lost_post_crash ℓ).
+  Proof. solve_proper. Qed.
+
+  Definition or_lost_post_crash_no_t ℓ (P : iProp Σ) :=
+    or_lost_post_crash ℓ (λ _, P).
+
+  (* A [dProp] version of [or_lost_post_crash]. *)
+  Definition or_lost_with_t ℓ (P : time → dProp Σ) : dProp Σ :=
+    ∃ CV,
+      ⎡ crashed_at CV ⎤ ∗
+      ((∃ t, ⌜CV !! ℓ = Some (MaxNat t)⌝ ∗ ⎡ persisted_loc ℓ 0 ⎤ ∗ P t) ∨
+        ⌜CV !! ℓ = None⌝).
+
+  (* The predicate [P] holds for [ℓ] or [ℓ] has been lost. *)
+  Definition or_lost ℓ (P : dProp Σ) : dProp Σ :=
+    or_lost_with_t ℓ (λ _, P).
+
+  Lemma or_lost_post_crash_lookup (CV : view) ℓ t P :
+    CV !! ℓ = Some (MaxNat t) →
+    crashed_at CV -∗
+    or_lost_post_crash ℓ P -∗
+    P t.
+  Proof.
+    iIntros (look) "crash".
+    iIntros "(% & crash' & [l|%])";
+      iDestruct (crashed_at_agree with "crash crash'") as %<-;
+      last congruence.
+    iDestruct "l" as (t' eq) "(per & P)".
+    by simplify_eq.
+  Qed.
+
+  (* Lemma or_lost_post_crash_no_t_lookup (CV : view) ℓ t P : *)
+  (*   CV !! ℓ = Some (MaxNat t) → *)
+  (*   crashed_at CV -∗ *)
+  (*   or_lost_post_crash_no_t ℓ P -∗ *)
+  (*   P. *)
+  (* Proof. apply or_lost_post_crash_lookup. Qed. *)
+
+  Lemma or_lost_post_crash_sep ℓ P Q :
+    or_lost_post_crash ℓ (λ t, P t ∗ Q t) ⊣⊢
+    or_lost_post_crash ℓ (λ t, P t) ∗ or_lost_post_crash ℓ (λ t, Q t).
+  Proof.
+    iSplit.
+    - iDestruct 1 as (?) "(#CV & [(%t & %look & #per & P & Q)|%look])".
+      * iSplitL "P"; iExists _; iFrame "CV"; iLeft; naive_solver.
+      * iSplitL; iExists _; naive_solver.
+    - iIntros "[(%CV & cr1 & [(%t1 & %look1 & #per & P)|%look1])
+                (%CV' & cr2 & [(%t2 & %look2 & #? & Q)|%look2])]";
+        iDestruct (crashed_at_agree with "cr1 cr2") as %eq;
+        simplify_eq.
+      * iExists _. iFrame. iLeft. iExists _. iFrame "∗#%".
+      * iExists _. iFrame. iRight. done.
+  Qed.
+
+  Lemma or_lost_post_crash_mono ℓ P Q :
+    (∀ t, ("#per" ∷ persisted_loc ℓ 0) -∗ P t -∗ Q t) -∗
+    or_lost_post_crash ℓ P -∗ or_lost_post_crash ℓ Q.
+  Proof.
+    iIntros "pToQ (%CV & crashed & disj)".
+    iExists CV. iFrame "crashed". iDestruct "disj" as "[(% & % & #per & P) | %lost]".
+    - iLeft. iExists _. iFrame "#". iSplitPure; first done.
+      iApply ("pToQ" with "[$] P").
+    - iRight. iFrame (lost).
+  Qed.
+
+  Global Instance or_lost_post_crash_fractional ℓ P :
+    (∀ t, Fractional (P t)) →
+    Fractional (λ q, or_lost_post_crash ℓ (λ t, P t q)).
+  Proof.
+    intros F q p.
+    rewrite -or_lost_post_crash_sep.
+    setoid_rewrite fractional.
+    done.
+  Qed.
+
+  (* Lemma or_lost_to_with_t ℓ P : or_lost ℓ P ⊣⊢ or_lost_with_t ℓ (λ _, P). *)
+  (* Proof. rewrite /or_lost. done. Qed. *)
+
+  Lemma or_lost_with_t_at ℓ (P : _ → dProp Σ) TV :
+    or_lost_post_crash ℓ (λ t, P t TV) -∗
+    (or_lost_with_t ℓ P) TV.
+  Proof.
+    iDestruct 1 as (CV) "[crash disj]".
+    iExists _. iFrame "crash disj".
+  Qed.
+
+  Lemma or_lost_with_t_sep ℓ (P Q : _ → dProp Σ) :
+    or_lost_with_t ℓ P ∗ or_lost_with_t ℓ Q ⊣⊢ or_lost_with_t ℓ (λ t, P t ∗ Q t)%I.
+  Proof.
+    iSplit.
+    - iIntros "[(%CV & crash & MP) (%CV' & crash' & MQ)]".
+      iDestruct (crashed_at_agree with "crash crash'") as %<-.
+      iExists CV. iFrame.
+      iDestruct "MP" as "[(% & % & #per & P)|%]"; iDestruct "MQ" as "[(% & % & #? & Q)|%]";
+        try (by iRight).
+      simplify_eq.
+      iLeft. iExists _. iFrame "∗#". done.
+    - iIntros "(%CV & #crash & [(% & % & #per & [P Q])|%])".
+      * iSplitL "P".
+        + iExists CV. iFrame "#". iLeft. iExists _. iFrame. done.
+        + iExists CV. iFrame "#". iLeft. iExists _. iFrame. done.
+      * iSplitL; iExists CV; iFrame "#%".
+  Qed.
+
+  Lemma or_lost_sep ℓ (P Q : dProp Σ) :
+    or_lost ℓ P ∗ or_lost ℓ Q ⊣⊢ or_lost ℓ (P ∗ Q)%I.
+  Proof. rewrite /or_lost. apply or_lost_with_t_sep. Qed.
+
+  Lemma or_lost_with_t_mono_strong ℓ (P Q : _ → dProp Σ) :
+    (∀ t, ("#per" ∷ ⎡ persisted_loc ℓ 0 ⎤) -∗ P t -∗ Q t) -∗
+    or_lost_with_t ℓ P -∗ or_lost_with_t ℓ Q.
+  Proof.
+    iIntros "pToQ (%CV & crashed & disj)".
+    iExists CV. iFrame "crashed". iDestruct "disj" as "[(% & % & #per & P) | %lost]".
+    - iLeft. iExists _. iFrame "#". iSplitPure; first done.
+      iApply ("pToQ" with "[$] P").
+    - iRight. iFrame (lost).
+  Qed.
+
+  Lemma or_lost_with_t_mono ℓ (P Q : _ → dProp Σ) :
+    (∀ t, P t -∗ Q t) -∗ or_lost_with_t ℓ P -∗ or_lost_with_t ℓ Q.
+  Proof.
+    iIntros "pToQ".
+    iApply (or_lost_with_t_mono_strong).
+    iIntros (?) "_". iApply "pToQ".
+  Qed.
+
+  Lemma or_lost_mono ℓ (P Q : dProp Σ) :
+    (P -∗ Q) -∗ or_lost ℓ P -∗ or_lost ℓ Q.
+  Proof. iIntros "I". iApply or_lost_with_t_mono. iIntros (_). done. Qed.
+
+  Lemma or_lost_embed ℓ P TV :
+    or_lost_post_crash_no_t ℓ P -∗ or_lost ℓ ⎡ P ⎤ TV.
+  Proof.
+    iDestruct 1 as (CV) "[crash disj]". iExists _. iFrame "crash". done.
+  Qed.
+
+  Lemma or_lost_get `{nvmDeltaG Σ} CV ℓ P :
+    is_Some (CV !! ℓ) → ⎡ crashed_at CV ⎤ -∗ or_lost ℓ P -∗ P.
+  Proof.
+    iIntros ([[t] look]) "crash (%CV' & crash' & [(% & ? & #per & $)|%look'])".
+    iDestruct (crashed_at_agree with "crash crash'") as %<-.
+    congruence.
+  Qed.
+
+  Lemma or_lost_with_t_get `{nvmDeltaG Σ} CV ℓ t P :
+    CV !! ℓ = Some (MaxNat t) → ⎡ crashed_at CV ⎤ -∗ or_lost_with_t ℓ P -∗ P t.
+  Proof.
+    rewrite /or_lost_with_t.
+    iIntros (look) "crash (%CV' & crash' & [(%t' & %look' & #per & P)|%look'])";
+    iDestruct (crashed_at_agree with "crash crash'") as %<-.
+    - simplify_eq. iFrame "P".
+    - congruence.
+  Qed.
+
+End or_lost_post_crash.
+
+Opaque or_lost.
+Opaque or_lost_post_crash.
